

Chapter 2

Interpolation and Approximation

Prepared by: **Sumanta Silwal**

Overview:

- Lagrange's Interpolation
- Newton's Divide and Difference Interpolation
- Cubic Spline Interpolation
- Curve Fitting

Interpolation

Let $f(x)$ be continuous function may be used to represent the $n + 1$ data values with passing $n + 1$ points. The process of computing the value of $f(x)$ or y for given x inside the given range is called Interpolation.

x	x_0	x_1	x_n
$f(x)$	$f(x_0)$	$f(x_1)$	$f(x_n)$

Then the process of finding the value of $f(x)$ corresponding to any value of x is called interpolation

Interpolation with unequal intervals

- Lagrange's interpolation
- Newton's divide and difference interpolation

Lagrange's Interpolation

Suppose $f(x)$ be a function with $f(x_0), f(x_1), f(x_2), \dots, f(x_n)$ corresponding to the values $x_0, x_1, x_2, \dots, x_n$ then the Lagrange's interpolation formula is given by:

$$f(x) = \frac{(x-x_1)(x-x_2)(x-x_3)}{(x_0-x_1)(x_0-x_2)(x_0-x_3)} \times f(x_0) + \frac{(x-x_0)(x-x_2)(x-x_3)}{(x_1-x_0)(x_1-x_2)(x_1-x_3)} \times f(x_1) + \frac{(x-x_0)(x-x_1)(x-x_3)}{(x_2-x_0)(x_2-x_1)(x_2-x_3)} \times f(x_2) + \frac{(x-x_0)(x-x_1)(x-x_2)}{(x_3-x_0)(x_3-x_1)(x_3-x_2)} \times f(x_3) + \dots + \frac{(x-x_0)(x-x_1) \dots (x-x_{n-1})}{(x_n-x_0)(x_n-x_1) \dots (x_n-x_{n-1})} \times f(x_n)$$

Solved Example 1:

Q. Use the Lagrange's interpolation formula to find the value of $f(x)$ at $x = 10$ ie $f(10)$ from the following data.

x	5	6	9	11
$f(x)$	12	13	14	16

Solution: $x_0 = 5, x_1 = 6, x_2 = 9, x_3 = 11$

$f(x_0) = 12, f(x_1) = 13, f(x_2) = 14, f(x_3) = 16$

By Lagrange's interpolation we have

$$f(x) = \frac{(x-x_1)(x-x_2)(x-x_3)}{(x_0-x_1)(x_0-x_2)(x_0-x_3)} \times f(x_0) + \frac{(x-x_0)(x-x_2)(x-x_3)}{(x_1-x_0)(x_1-x_2)(x_1-x_3)} \times f(x_1) + \frac{(x-x_0)(x-x_1)(x-x_3)}{(x_2-x_0)(x_2-x_1)(x_2-x_3)} \times f(x_2) + \frac{(x-x_0)(x-x_1)(x-x_2)}{(x_3-x_0)(x_3-x_1)(x_3-x_2)} \times f(x_3)$$

$$\therefore f(10) = \frac{(10-6)(10-9)(10-11)}{(5-6)(5-9)(5-11)} \times 12 + \frac{(10-5)(10-9)(10-11)}{(6-5)(6-9)(6-11)} \times 13 + \frac{(10-5)(10-6)(10-11)}{(9-5)(9-6)(9-11)} \times 14 + \frac{(10-5)(10-6)(10-9)}{(11-5)(11-6)(11-9)} \times 16$$

$$= 2 - 4.3333 + 11.6666 + 5.3333$$

$$= 14.6666$$

Exercise:

1. Use Lagrange interpolation to estimate the square of 3.25 if

X	1	2	3	4	5
$f(x) = x^2$	1	4	9	16	25

2. Find the missing value from the following table using Lagrange interpolation.

X	1	3	6.5	10
$f(x)$	23	61	?	203

X	-2	-1	0	1	6
$f(x) = x^2$	-20	?	2	?	70

Lagrange's Interpolation Algorithm

1. Read the number of data 'n'
2. Read the value at which value is needed(say x)
3. Read the available data points x and f(x)
4. Initialize sum=0
5. for i=0 to n
 initialize L[i]=1.
 for j=0 to n
 if(i!=j)
 $L[i]=L[i]*(x-x[j])/(x[i]-x[j])$
 end if
 end for
5. sum=sum+L[i]*f[i]
 end for
7. Print interpolation value "sum" at x
8. END

Newton's Divide and Difference Interpolation

Let $f(x)$ be a function with $f(x_0), f(x_1), f(x_2), \dots, f(x_n)$ corresponding to values $x_0, x_1, x_2, \dots, x_n$ then Newton's divide difference interpolation is given by;

$$f(x) = f(x_0) + (x - x_0)f[x_0, x_1] + (x - x_0)(x - x_1)f[x_0, x_1, x_2] \\ + \dots \dots \dots (x - x_0)(x - x_1) \dots \dots (x - x_n)f[x_0, x_1, \dots \dots x_n]$$

or, It can be written as;

$$f(x) = f_0 + (x - x_0)\Delta f_0 + (x - x_0)(x - x_1)\Delta^2 f_0 + (x - x_0)(x - x_1)(x - x_2)\Delta^3 f_0 + \dots \dots$$

Now, we can construct the divide and difference table as follows

x	f	Δf	$\Delta^2 f$	$\Delta^3 f$
x_0	f_0			
		$\frac{f_1 - f_0}{x_1 - x_0} = \Delta f_0$		
x_1	f_1		$\frac{\Delta f_1 - \Delta f_0}{x_2 - x_0} = \Delta^2 f_0$	
		$\frac{f_2 - f_1}{x_2 - x_1} = \Delta f_1$		$\frac{\Delta^2 f_1 - \Delta^2 f_0}{x_3 - x_0} = \Delta^3 f_0$
x_2	f_2		$\frac{\Delta f_2 - \Delta f_1}{x_3 - x_1} = \Delta^2 f_1$	
		$\frac{f_3 - f_2}{x_3 - x_2} = \Delta f_2$		
x_3	f_3			

Solved Example 1:

Q. Using Newton's divide difference interpolation estimate the value of $f(x)$ at $x=4$ for the function defined below.

x	0	2	3	6
f	648	704	729	792

Solution: The divide difference table for the given data;

x	f	Δf	$\Delta^2 f$	$\Delta^3 f$
0	648			
		$\frac{704 - 648}{2 - 0} = 28$		
2	704		$\frac{25 - 28}{3 - 0} = -1$	
		$\frac{729 - 704}{3 - 2} = 25$		$\frac{-1 + 1}{6 - 0} = 0$
3	729		$\frac{21 - 25}{6 - 2} = -1$	
		$\frac{792 - 729}{6 - 3} = 21$		
6	792			

We have,

$$f(x) = f(x_0) + (x - x_0)f[x_0, x_1] + (x - x_0)(x - x_1)f[x_0, x_1, x_2] + (x - x_0)(x - x_1)(x - x_2)f[x_0, x_1, x_2, x_3]$$

$$= 648 + (x - 0)28 + (x - 0)(x - 2)(-1) + 0$$

$$\therefore f(4) = 648 + (4 - 0)28 + (4 - 0)(4 - 2)(-1)$$

$$= 752$$

Exercise:

1. Using Newton's divide difference interpolation estimate the value of $f(x)$ at $x=1.75$ for the function defined below.

x	<i>1.1</i>	<i>2.0</i>	<i>3.5</i>	<i>5</i>	<i>7.1</i>
f	<i>0.6981</i>	<i>1.4715</i>	<i>2.1287</i>	<i>2.0521</i>	<i>1.4480</i>

Interpolation with equal intervals

- Newton's forward interpolation
- Newton's backward interpolation

Newton's forward interpolation

Newton's forward interpolation formula

$$y_s = y_0 + s\Delta y_0 + \frac{s(s-1)}{2!}\Delta^2 y_0 + \frac{s(s-1)(s-2)}{3!}\Delta^3 y_0 + \frac{s(s-1)(s-2)(s-3)}{4!}\Delta^4 y_0 + \dots$$

Where $s = \frac{x_s - x_0}{h}$, x_s = value at which interpolation is to be found
 x_0 = initial value, h = interval of 'x'

x	y	Δy	$\Delta^2 y$	$\Delta^3 y$
x_0	y_0			
		$\Delta y_0 = y_1 - y_0$		
x_1	y_1		$\Delta^2 y_0 = \Delta y_1 - \Delta y_0$	
		$\Delta y_1 = y_2 - y_1$		$\Delta^3 y_0 = \Delta^2 y_1 - \Delta^2 y_0$
x_2	y_2		$\Delta^2 y_1 = \Delta y_2 - \Delta y_1$	
		$\Delta y_2 = y_3 - y_2$		
x_3	y_3			

Newton's backward interpolation

Newton's backward interpolation formula

$$y_s = y_n + s\nabla y_n + \frac{s(s+1)}{2!}\nabla^2 y_n + \frac{s(s+1)(s+2)}{3!}\nabla^3 y_n + \frac{s(s+1)(s+2)(s+3)}{4!}\nabla^4 y_n + \dots$$

Where $s = \frac{x_s - x_n}{h}$, x_s = value at which interpolation is to be found
 x_n = final value, h = interval of 'x'

x	y	∇y	$\nabla^2 y$	$\nabla^3 y$
x_0	y_0			
		$\nabla y_0 = y_1 - y_0$		
x_1	y_1		$\nabla^2 y_0 = \nabla y_1 - \nabla y_0$	
		$\nabla y_1 = y_2 - y_1$		$\nabla^3 y_0 = \nabla^2 y_1 - \nabla^2 y_0$
x_2	y_2		$\nabla^2 y_1 = \nabla y_2 - \nabla y_1$	
		$\nabla y_2 = y_3 - y_2$		
x_3	y_3			

When to use forward/Backward interpolation?

- **Forward Interpolation:** When data is given in ascending order or the required point is close to the starting point of the table.
- **Backward interpolation:** when the data is given in descending order or the required point is close to the end point of the table.

Solved Example 1:

Q. Using Newton's forward interpolation formula for the given table to evaluate $f(5)$.

<i>x</i>	<i>4</i>	<i>6</i>	<i>8</i>	<i>10</i>
<i>y</i>	<i>1</i>	<i>3</i>	<i>8</i>	<i>16</i>

Solution: The difference table for the given data;

x	y	Δy	$\Delta^2 y$	$\Delta^3 y$
4	1			
		2		
6	3		3	
		5		0
8	8		3	
		8		
10	16			

Here, $x_s=5$, $x_0=4$, and $h= 2$

$$s = \frac{x_s - x_0}{h} = \frac{5-4}{2} = 0.5$$

Newton's forward interpolation formula

$$\begin{aligned}y_s &= y_0 + s\Delta y_0 + \frac{s(s-1)}{2!}\Delta^2 y_0 + \frac{s(s-1)(s-2)}{3!}\Delta^3 y_0 \\y_5 &= 1 + (0.5)(2) + \frac{0.5(0.5-1)}{2!}(3) + \frac{0.5(0.5-1)(0.5-2)}{3!}(0) \\&= 1 + 1 - 0.375 + 0 \\&= 1.625\end{aligned}$$

$$\therefore f(5) = 1.625$$

Solved Example 2:

Q. Using Newton's backward interpolation formula for the given table to evaluate $f(17)$.

x	0	5	10	15	20
$f(x)$	1.0	1.6	3.8	8.2	15.4

Solution: The difference table for the given data;

x	$y=f(x)$	∇y	$\nabla^2 y$	$\nabla^3 y$	$\nabla^4 y$
0	1.0				
		0.6			
5	1.6		1.6		
		2.2		0.6	
10	3.8		2.2		0
		4.4		0.6	
15	8.2		2.8		
		7.2			
20	15.4				

Here, $x_s=17$, $x_n=20$, and $h= 5$

$$s = \frac{x_s - x_n}{h} = \frac{17 - 20}{5} = -0.6$$

Newton's backward interpolation formula

$$y_s = y_n + s\nabla y_n + \frac{s(s+1)}{2!}\nabla^2 y_n + \frac{s(s+1)(s+2)}{3!}\nabla^3 y_n + \frac{s(s+1)(s+2)(s+3)}{4!}\nabla^4 y_n$$
$$\begin{aligned}\therefore y_{17} &= 15.4 + (-0.6)(7.2) + \frac{(-0.6)(-0.6+1)}{2!}(2.8) + \frac{(-0.6)(-0.6+1)(-0.6+2)}{3!}(0.6) + 0 \\ &= 15.4 - 4.32 - 0.336 - 0.0336 + 0 \\ &= 10.7104\end{aligned}$$

$$\therefore y_{17} = 10.7104$$

Exercise:

1. Using Newton's forward difference formula estimate the value of $f(x)$ at $x=3.6$ for the function defined below.

x	2	2.5	3	3.5	4	4.5
$f(x)$	1.43	1.03	0.76	0.6	0.48	0.39

2. Using Newton's backward difference formula estimate the value of $\ln(3.5)$ for the function defined below.

x	1.0	2.0	3.0	4.0
$\ln(x)$	0.0	0.6931	1.0986	1.3863

Cubic Spline Interpolation

Cubic interpolation works by constructing the (cubic) polynomial in pieces. Given n points will construct $n-1$ different (cubic) polynomials. These polynomials have consistent derivatives at the end points.

Formula

Formula 1

$$h_i a_{i-1} + 2a_i(h_i + h_{i+1}) + h_{i+1} a_{i+1} = 6 \left[\frac{f_{i+1} - f_i}{h_{i+1}} - \frac{f_i - f_{i-1}}{h_i} \right] \dots \dots \dots (1)$$

Where $a_0 = a_n = 0$

Formula 2

$$s_i(x) = \frac{a_{i-1}}{6h_i} (h_i^2 U_i - U_i^3) + \frac{a_i}{6h_i} (U_{i-1}^3 - h_i^2 U_{i-1}) + \frac{1}{h_i} (f_i U_{i-1} - f_{i-1} U_i) \dots \dots \dots (2)$$

$$h_i = x_i - x_{i-1} \quad \text{and} \quad U_i = x - x_i$$

Evaluate equation 1 ***for i= 1to n-1***

Evaluate equation 2 at ***i=a*** value given by position interval

Solved Example 1:

Q. Estimate the functional value of f at $x=7$ using cubic splines from given table.

x	4	9	16
f	2	3	4

Solution:

$$h_1 = x_1 - x_0 = 9 - 4 = 5$$

$$h_2 = x_2 - x_1 = 16 - 9 = 7$$

$$f_0 = 2, f_1 = 3, f_2 = 4$$

$$a_0 = a_2 = 0$$

We have:

$$h_i a_{i-1} + 2a_i(h_i + h_{i+1}) + h_{i+1} a_{i+1} = 6 \left[\frac{f_{i+1} - f_i}{h_{i+1}} - \frac{f_i - f_{i-1}}{h_i} \right]$$

For $i = 1$

$$h_1 a_0 + 2a_1(h_1 + h_2) + h_2 a_2 = 6 \left[\frac{f_2 - f_1}{h_2} - \frac{f_1 - f_0}{h_1} \right]$$

$$0 + 2a_1(5 + 7) + 0 = 6 \left[\frac{4-3}{7} - \frac{3-2}{5} \right]$$

$$24a_1 = 6 \left[\frac{1}{7} - \frac{1}{5} \right]$$

$$\mathbf{a_1 = -0.0143}$$

Again from second formula,

$$s_i(x) = \frac{a_{i-1}}{6h_i} (h_i^2 U_i - U_i^3) + \frac{a_i}{6h_i} (U_{i-1}^3 - h_i^2 U_{i-1}) + \frac{1}{h_i} (f_i U_{i-1} - f_{i-1} U_i)$$

$$s_1(x) = \frac{a_0}{6h_1} (h_1^2 U_1 - U_1^3) + \frac{a_1}{6h_1} (U_0^3 - h_1^2 U_0) + \frac{1}{h_1} (f_1 U_0 - f_0 U_1)$$

$$U_0 = x - x_0 = x - 4$$

$$U_1 = x - x_1 = x - 9$$

$$\therefore s_1(7) = 0 + \frac{-0.0143}{6 \times 5} [(7 - 4)^3 - 5^2(7 - 4)] + \frac{1}{5} [3(7 - 4) - 2(7 - 9)]$$

$$= 2.6229$$

Curve Fitting

Curve fitting is the process of introducing mathematical relationship between dependent and independent variables in the form of an equation for a given set of data.

- Linear Curve Fitting
- Non - Linear Curve Fitting

Linear Curve Fitting

$y = a + bx$ --- (i) where ***a*** and ***b*** are constants and are unknown

The normal equation of (i) is

$$\sum y_i = na + b \sum x_i \quad \text{--- (ii)}$$

$$\sum x_i y_i = a \sum x_i + b \sum x_i^2 \quad \text{--- (iii)}$$

Solving equation (ii & iii) we can determine the constants a and b.

$$b = \frac{n \sum x_i y_i - \sum x_i \sum y_i}{n \sum x_i^2 - (\sum x_i)^2}$$
$$a = \frac{\sum y_i}{n} - b \frac{\sum x_i}{n} = \bar{y} - b\bar{x}$$

Solved Example 1:

Q. Fit a straight line to the following set of data.

<i>x</i>	<i>1</i>	<i>2</i>	<i>3</i>	<i>4</i>	<i>5</i>
<i>y</i>	<i>3</i>	<i>4</i>	<i>5</i>	<i>6</i>	<i>8</i>

Solution:

<i>x</i>	<i>y</i>	<i>x</i>²	<i>xy</i>
1	3	1	3
2	4	4	8
3	5	9	15
4	6	16	24
5	8	25	40
$\sum x = 15$	$\sum y = 26$	$\sum x^2 = 55$	$\sum xy = 90$

We have:

$$b = \frac{n \sum x_i y_i - \sum x_i \sum y_i}{n \sum x_i^2 - (\sum x_i)^2} = \frac{5 \times 90 - 15 \times 26}{5 \times 55 - 15^2} = 1.2$$

$$a = \frac{\sum y_i}{n} - b \frac{\sum x_i}{n} = \frac{26}{5} - 1.2 \times \frac{15}{5} = 1.6$$

The linear equation is:

$$y = a + bx$$

$$\therefore \mathbf{y = 1.6 + 1.2\ x}$$

Non-Linear Curve Fitting

a. Exponential Function

Let the curve be $y = ae^{bx}$ ---(i)

Taking log on both sides

$$\log y = \log a + (b \cdot \log e) \cdot x$$

$$Y = A + Bx \text{ --- (ii) } [\because \log e = 1]$$

Where,

$$Y = \log y$$

$$B = \log e \cdot b$$

$$A = \log a$$

Solved Example 1:

Q. Fit the following set of data to the curve of the form $y = ae^{bx}$

<i>x</i>	<i>2</i>	<i>4</i>	<i>6</i>	<i>8</i>	<i>10</i>	<i>12</i>
<i>y</i>	<i>16</i>	<i>17.1</i>	<i>8.7</i>	<i>6.4</i>	<i>4.7</i>	<i>2.6</i>

Solution:

Let the curve be $y = ae^{bx}$ ---(i)

Taking log on both sides

$$\log y = \log a + x \log b$$

$$Y = A + Bx \text{ ----(ii) } [\because \log e = 1]$$

Where,

$$Y = \log y$$

$$B = \log b$$

$$A = \log a$$

We have,

X	y	Y=log y	X ²	XY
2	16	1.20412	4	2.40824
4	11.1	1.04532	16	4.18128
6	8.7	0.93952	36	5.63712
8	6.4	0.80618	64	6.44944
10	4.7	0.67209	100	6.7209
12	2.6	0.41497	144	4.97964
$\sum X = 42$		$\sum Y = 5.0822$	$\sum X^2 = 364$	$\sum XY = 30.37662$

$$B = \frac{n \sum x_i y_i - \sum x_i \sum y_i}{n \sum x_i^2 - (\sum x_i)^2} = \frac{6 \times 30.37662 - 42 \times 5.0822}{6 \times 364 - 42^2} = -0.07427$$

$$A = \frac{\sum y_i}{n} - B \frac{\sum x_i}{n} = \frac{5.0822}{6} - (-0.07427) \times \frac{42}{6} = 1.36692$$

Now,

$$a = \text{antilog}(1.36692) = 23.27662$$

$$b = (-0.07427)/\log e = -0.1710$$

So the equation (i) becomes,

$$\therefore \mathbf{y = 23.27662e^{-0.1710x}}$$

*Thank
you!*